CC/Typed/CanonicalForm.lean
@@ -16,10 +16,10 @@ import CC.Typed.TypeSubst
 namespace CC
 
 theorem Typed.cf_fun' :
-  t0 = Term.abs T' t ->
-  T0 = CType.capt C (PType.arr T U) ->
+  t0 = Term.abs D' T' t ->
+  T0 = CType.capt C (PType.arr D T U) ->
   Typed Γ t0 Ct T0 ->
-  ∃ C', Typed (Ctx.extend_var Γ T) t C' U := by
+  ∃ C', Typed (Ctx.extend_var Γ D T) t C' U := by
   intro he1 he2 h
   induction h <;> try (solve | cases he1 | cases he2)
   case abs h hd ih =>
@@ -46,8 +46,8 @@ theorem Typed.cf_fun' :
       repeat trivial
 
 theorem Typed.cf_fun :
-  Typed Γ (Term.abs T' t) Ct (CType.capt C (PType.arr T U)) ->
-  ∃ C', Typed (Ctx.extend_var Γ T) t C' U := by
+  Typed Γ (Term.abs D' T' t) Ct (CType.capt C (PType.arr D T U)) ->
+  ∃ C', Typed (Ctx.extend_var Γ D T) t C' U := by
   intro h
   apply Typed.cf_fun' <;> trivial
 
